updates

Veritas.Verifier.Blum.fsti
@@ -9,6 +9,7 @@ open Veritas.MultiSetHash
 open Veritas.SeqAux
 open Veritas.Verifier
 open Veritas.Verifier.Global
+open Veritas.Verifier.Thread
 open Veritas.Verifier.TSLog
 
 module E=Veritas.EAC
@@ -17,36 +18,6 @@ module MS=Veritas.MultiSet
 module MH=Veritas.MultiSetHash
 module TL=Veritas.Verifier.TSLog
 module VG = Veritas.Verifier.Global
-
-(* global add sequence *)
-val g_add_seq (gl: VG.verifiable_log): seq (ms_hashfn_dom)
-
-(* multiset derived from all the blum adds in gl *)
-let g_add_set (gl: VG.verifiable_log): mset ms_hashfn_dom =
-  seq2mset (g_add_seq gl)
-
-(* the hadd that the verifier computes is the multiset hash of all the adds *)
-val lemma_g_hadd_correct (gl: VG.verifiable_log):
-  Lemma (VG.hadd gl = ms_hashfn (g_add_seq gl))
-
-(* a single sequence containing all the blum evicts *)
-val g_evict_seq (gl: VG.verifiable_log): seq ms_hashfn_dom 
-
-let g_evict_set (gl: VG.verifiable_log): mset ms_hashfn_dom = 
-  seq2mset (g_evict_seq gl)
-
-(* the global evict set is a set (not a multiset) *)
-val g_evict_set_is_set (gl: VG.verifiable_log): 
-  Lemma (is_set (g_evict_set gl))
-
-val lemma_ghevict_correct (gl: VG.verifiable_log):
-  Lemma (VG.hevict gl = ms_hashfn (g_evict_seq gl))
-
-(* get the blum add element from an index *)
-let blum_add_elem (e:vlog_entry {is_blum_add e}):
-  ms_hashfn_dom = 
-  match e with
-  | AddB r t j -> MHDom r t j
 
 (* sequence of blum adds in the time sequenced log *)
 val ts_add_seq (itsl: its_log): seq ms_hashfn_dom
@@ -57,7 +28,7 @@ let ts_add_set (itsl: its_log): mset ms_hashfn_dom
 
 val lemma_add_elem_correct (itsl: its_log) (i: I.seq_index itsl):
   Lemma (requires (is_blum_add (I.index itsl i)))
-        (ensures (contains (blum_add_elem (index itsl i)) (ts_add_set itsl)))
+        (ensures (contains (blum_add_elem (I.index itsl i)) (ts_add_set itsl)))
 
 (* sequence of blum adds restricted to key k *)
 val ts_add_seq_key (itsl: its_log) (k:key): seq ms_hashfn_dom
@@ -72,16 +43,16 @@ val lemma_ts_add_set_correct (itsl: its_log):
 
 (* if the tail element is a blum add, then the add set is obtained by adding that 
  * blum add to the prefix *)
-val lemma_ts_add_set_key_extend (itsl: its_log {length itsl > 0}):
+val lemma_ts_add_set_key_extend (itsl: its_log {I.length itsl > 0}):
   Lemma (requires (is_blum_add (I.telem itsl)))
-        (ensures (ts_add_set_key itsl (key_of (index itsl (length itsl - 1))) == 
-                  add_elem (ts_add_set_key (I.prefix itsl (length itsl - 1))
-                                           (key_of (index itsl (length itsl - 1))))
+        (ensures (ts_add_set_key itsl (key_of (I.index itsl (I.length itsl - 1))) == 
+                  add_elem (ts_add_set_key (I.prefix itsl (I.length itsl - 1))
+                                           (key_of (I.index itsl (I.length itsl - 1))))
                            (blum_add_elem (I.telem itsl))))
 
 val lemma_ts_add_set_contains_add_elem (itsl: its_log) (i:I.seq_index itsl):
-  Lemma (requires (is_blum_add (index itsl i)))
-        (ensures (MS.contains (blum_add_elem (index itsl i)) (ts_add_set itsl)))
+  Lemma (requires (is_blum_add (I.index itsl i)))
+        (ensures (MS.contains (blum_add_elem (I.index itsl i)) (ts_add_set itsl)))
 
 val lemma_ts_add_set_key_contains_only (itsl: its_log) (k:key) (be: ms_hashfn_dom):
   Lemma (requires (MS.contains be (ts_add_set_key itsl k)))
@@ -89,15 +60,15 @@ val lemma_ts_add_set_key_contains_only (itsl: its_log) (k:key) (be: ms_hashfn_do
 
 val some_add_elem_idx (itsl: its_log) 
   (be: ms_hashfn_dom{MS.contains be (ts_add_set itsl)}): 
-  (i:(I.seq_index itsl){is_blum_add (index itsl i) /\
-                      be = blum_add_elem (index itsl i)})
+  (i:(I.seq_index itsl){is_blum_add (I.index itsl i) /\
+                      be = blum_add_elem (I.index itsl i)})
 
 (* get the blum evict element from an index *)
-val blum_evict_elem (itsl: its_log) (i:I.seq_index itsl{is_evict_to_blum (index itsl i)}):
-  (e:ms_hashfn_dom{MH.key_of e = key_of (index itsl i)})
+val blum_evict_elem (itsl: its_log) (i:I.seq_index itsl{is_evict_to_blum (I.index itsl i)}):
+  (e:ms_hashfn_dom{MH.key_of e = key_of (I.index itsl i)})
 
-val lemma_index_blum_evict_prefix (itsl: its_log) (i:nat{i <= length itsl}) (j:nat{j < i}):
-  Lemma (requires (is_evict_to_blum (index itsl j)))
+val lemma_index_blum_evict_prefix (itsl: its_log) (i:nat{i <= I.length itsl}) (j:nat{j < i}):
+  Lemma (requires (is_evict_to_blum (I.index itsl j)))
         (ensures (blum_evict_elem itsl j = blum_evict_elem (I.prefix itsl i) j))
         [SMTPat (blum_evict_elem (I.prefix itsl i) j)]
 
@@ -122,35 +93,35 @@ val lemma_ts_evict_set_correct (itsl: its_log):
 (* if the tail element is not an evict, the evict set is the same as the evict 
  * set of the length - 1 prefix 
  *)
-val lemma_ts_evict_set_key_extend2 (itsl: its_log {length itsl > 0}):
-  Lemma (requires (not (is_evict_to_blum (index itsl (length itsl - 1)))))
-        (ensures (ts_evict_set_key itsl (key_of (index itsl (length itsl - 1))) == 
-                  ts_evict_set_key (I.prefix itsl (length itsl - 1))
-                                           (key_of (index itsl (length itsl - 1)))))
+val lemma_ts_evict_set_key_extend2 (itsl: its_log {I.length itsl > 0}):
+  Lemma (requires (not (is_evict_to_blum (I.index itsl (I.length itsl - 1)))))
+        (ensures (ts_evict_set_key itsl (key_of (I.index itsl (I.length itsl - 1))) == 
+                  ts_evict_set_key (I.prefix itsl (I.length itsl - 1))
+                                           (key_of (I.index itsl (I.length itsl - 1)))))
 
 (* since evict_set is a pure set (not a multiset) we can identify the unique index 
  * for each element of the set *)
 val index_blum_evict (itsl: its_log) (e: ms_hashfn_dom {contains e (ts_evict_set itsl)}):
-  (i:I.seq_index itsl{is_evict_to_blum (index itsl i) /\ 
+  (i:I.seq_index itsl{is_evict_to_blum (I.index itsl i) /\ 
                     blum_evict_elem itsl i = e})
 
 (* if the blum add occurs in the blum evict set, its index is earlier *)
-val lemma_evict_before_add (itsl: its_log) (i:I.seq_index itsl{is_blum_add (index itsl i)}):
+val lemma_evict_before_add (itsl: its_log) (i:I.seq_index itsl{is_blum_add (I.index itsl i)}):
   Lemma (requires True)
-        (ensures (not (contains (blum_add_elem (index itsl i)) (ts_evict_set itsl)) \/
-                  index_blum_evict itsl (blum_add_elem (index itsl i)) < i))
+        (ensures (not (contains (blum_add_elem (I.index itsl i)) (ts_evict_set itsl)) \/
+                  index_blum_evict itsl (blum_add_elem (I.index itsl i)) < i))
 
 (* a slightly different version of of the previous lemma - the count of an add element 
  * in the evict set is the same in the prefix as the full sequence *)
-val lemma_evict_before_add2 (itsl: its_log) (i:I.seq_index itsl{is_blum_add (index itsl i)}):
+val lemma_evict_before_add2 (itsl: its_log) (i:I.seq_index itsl{is_blum_add (I.index itsl i)}):
    Lemma (requires True)
-         (ensures (MS.mem (blum_add_elem (index itsl i)) (ts_evict_set itsl) =
-                   MS.mem (blum_add_elem (index itsl i)) (ts_evict_set (I.prefix itsl i))))
+         (ensures (MS.mem (blum_add_elem (I.index itsl i)) (ts_evict_set itsl) =
+                   MS.mem (blum_add_elem (I.index itsl i)) (ts_evict_set (I.prefix itsl i))))
 
 val lemma_evict_before_add3 (itsl: its_log) (i: I.seq_index itsl) (j:I.seq_index itsl):
-  Lemma (requires (is_blum_add (index itsl i) /\
-                   is_evict_to_blum (index itsl j) /\
-                   blum_add_elem (index itsl i) = blum_evict_elem itsl j))
+  Lemma (requires (is_blum_add (I.index itsl i) /\
+                   is_evict_to_blum (I.index itsl j) /\
+                   blum_add_elem (I.index itsl i) = blum_evict_elem itsl j))
         (ensures (j < i))
 
 (* for an eac ts log, if the eac state of a key k is instore, the count of blum evicts 
@@ -172,17 +143,17 @@ val lemma_mem_key_evict_set_same (itsl: its_log) (be: ms_hashfn_dom):
   Lemma (mem be (ts_evict_set itsl) = mem be (ts_evict_set_key itsl (MH.key_of be)))
 
 (* the count of an element can only decrease in a prefix of itsl *)
-val lemma_mem_monotonic (be:ms_hashfn_dom) (itsl: its_log) (i:nat{i <= length itsl}):
+val lemma_mem_monotonic (be:ms_hashfn_dom) (itsl: its_log) (i:nat{i <= I.length itsl}):
   Lemma (mem be (ts_evict_set itsl) >= mem be (ts_evict_set (I.prefix itsl i)) /\
          mem be (ts_add_set itsl) >= mem be (ts_add_set (I.prefix itsl i)))
 
 (* the next add of a blum evict is a blum add of the same "element" *)
 val lemma_blum_evict_add_same (itsl: TL.eac_log) (i:I.seq_index itsl):
-  Lemma (requires (is_evict_to_blum (index itsl i) /\
-                   TL.has_next_add_of_key itsl i (key_of (index itsl i))))
-        (ensures (is_blum_add (index itsl (TL.next_add_of_key itsl i (key_of (index itsl i)))) /\
+  Lemma (requires (is_evict_to_blum (I.index itsl i) /\
+                   TL.has_next_add_of_key itsl i (key_of (I.index itsl i))))
+        (ensures (is_blum_add (I.index itsl (TL.next_add_of_key itsl i (key_of (I.index itsl i)))) /\
                   blum_evict_elem itsl i =                                   
-                  blum_add_elem (index itsl (TL.next_add_of_key itsl i (key_of (index itsl i))))))
+                  blum_add_elem (I.index itsl (TL.next_add_of_key itsl i (key_of (I.index itsl i))))))
 
 let to_blum_elem (s: eac_state{EACEvictedBlum? s}) (k:key): ms_hashfn_dom = 
   match s with
@@ -192,14 +163,14 @@ let to_blum_elem (s: eac_state{EACEvictedBlum? s}) (k:key): ms_hashfn_dom =
 val lemma_eac_evicted_blum_implies_previous_evict (itsl: its_log) (k:key):
   Lemma (requires (is_eac_state_evicted_blum itsl k))
         (ensures (has_some_entry_of_key itsl k /\
-                  is_evict_to_blum (index itsl (last_idx_of_key itsl k)) /\
+                  is_evict_to_blum (I.index itsl (last_idx_of_key itsl k)) /\
                   blum_evict_elem itsl (last_idx_of_key itsl k) = 
                   to_blum_elem (eac_state_of_key itsl k) k))
 
 (* if we provide two indexes having the same add element then the membership of the element in the 
  * add set is at least two *)
 val lemma_add_set_mem (itsl: its_log) (i: I.seq_index itsl) (j:I.seq_index itsl{j <> i}):
-  Lemma (requires (is_blum_add (index itsl i) /\
-                   is_blum_add (index itsl j) /\
-                   blum_add_elem (index itsl i) = blum_add_elem (index itsl j)))
-        (ensures (MS.mem (blum_add_elem (index itsl i)) (ts_add_set itsl) >= 2))
+  Lemma (requires (is_blum_add (I.index itsl i) /\
+                   is_blum_add (I.index itsl j) /\
+                   blum_add_elem (I.index itsl i) = blum_add_elem (I.index itsl j)))
+        (ensures (MS.mem (blum_add_elem (I.index itsl i)) (ts_add_set itsl) >= 2))
